src/Common/CommonStreams.v
@@ -1,0 +1,92 @@
+From Coq Require Import Setoid.
+From Coq Require Import Streams.
+
+(** Additional streams utilities *)
+
+Section decompose.
+  Context {A : Type}.
+
+  Definition Stream_decompose (s : Stream A) : Stream A :=
+    match s with Cons a sa => Cons a sa end.
+
+  Lemma Stream_decompose_thm : forall (s : Stream A),
+      s = Stream_decompose s.
+  Proof.
+    intros s. case s; simpl; trivial.
+  Qed.
+End decompose.
+
+Section map.
+  Context {A B : Type}.
+
+  Variable (f : (A -> B)).
+
+  Lemma map_Cons : forall a (sa : Stream A),
+      (map f (Cons a sa)) = (Cons (f a) (map f sa)).
+  Proof.
+    intros a sa; simpl.
+    rewrite Stream_decompose_thm at 1; reflexivity.
+  Qed.
+End map.
+
+Section map2.
+  Context {A B C : Type}.
+
+  Variable (f : (A -> B -> C)).
+
+  CoFixpoint map2 (sa : Stream A) (sb : Stream B) : Stream C :=
+    match sa, sb with
+    | Cons hda tla, Cons hdb tlb =>
+      Cons (f hda hdb) (map2 tla tlb)
+    end.
+
+  Lemma map2_Cons : forall a b (sa : Stream A) (sb : Stream B),
+      (map2 (Cons a sa) (Cons b sb)) = (Cons (f a b) (map2 sa sb)).
+  Proof.
+    intros a b sa sb; simpl.
+    rewrite Stream_decompose_thm at 1; reflexivity.
+  Qed.
+
+  Lemma map2_hd : forall (sa : Stream A) (sb : Stream B),
+      f (hd sa) (hd sb) = hd (map2 sa sb).
+  Proof. intros [a sa] [b sb]; reflexivity. Qed.
+
+  Lemma map2_tl : forall (sa : Stream A) (sb : Stream B),
+      map2 (tl sa) (tl sb) = tl (map2 sa sb).
+  Proof. intros [a sa] [b sb]; reflexivity. Qed.
+
+  Lemma Str_nth_tl_map2 : forall n (sa : Stream A) (sb : Stream B),
+      Str_nth_tl n (map2 sa sb) = map2 (Str_nth_tl n sa) (Str_nth_tl n sb).
+  Proof.
+    induction n; intros sa sb; simpl.
+    - reflexivity.
+    - destruct sa. destruct sb. simpl.
+      auto.
+  Qed.
+
+  Lemma Str_nth_map2 : forall n (sa : Stream A) (sb : Stream B),
+      Str_nth n (map2 sa sb) = f (Str_nth n sa) (Str_nth n sb).
+  Proof.
+    unfold Str_nth.
+    induction n; intros [hda tla] [hdb tlb].
+    - reflexivity.
+    - simpl. auto.
+  Qed.
+End map2.
+
+Add Parametric Relation A : (Stream A) (@EqSt A)
+    reflexivity proved by (@EqSt_reflex A)
+    symmetry proved by (@sym_EqSt A)
+    transitivity proved by (@trans_EqSt A)
+      as EqStrel.
+
+Add Parametric Morphism A B C f : (@map2 A B C f)
+    with signature (@EqSt A) ==> (@EqSt B) ==> (@EqSt C) as map2_EqSt.
+Proof.
+  cofix map2_EqSt.
+  intros [? ?] [? ?] Eqa [? ?] [? ?] Eqb.
+  inversion Eqa; simpl in *; subst; clear Eqa.
+  inversion Eqb; simpl in *; subst; clear Eqb.
+  rewrite map2_Cons. rewrite map2_Cons.
+  constructor; simpl; auto.
+Qed.
