src/Lustre/LClockSemantics.v
@@ -1,0 +1,214 @@
+From Coq Require Import List.
+Import List.ListNotations.
+Open Scope list_scope.
+
+From Coq Require Import Streams.
+From Coq Require Import Sorting.Permutation.
+From Coq Require Import Setoid.
+From Coq Require Import Morphisms.
+
+From Coq Require Import FSets.FMapPositive.
+From Velus Require Import Common.
+From Velus Require Import CommonList.
+From Velus Require Import Environment.
+From Velus Require Import Operators.
+From Velus Require Import Clocks.
+From Velus Require Import Lustre.LSyntax Lustre.LClocking Lustre.LOrdered Lustre.LSemantics.
+From Velus Require Import CoindStreams.
+
+Local Set Warnings "-masking-absolute-name".
+Module Type LCLOCKSEMANTICS
+       (Import Ids : IDS)
+       (Import Op : OPERATORS)
+       (Import OpAux : OPERATORS_AUX Op)
+       (Import Syn : LSYNTAX Ids Op)
+       (Import Clo : LCLOCKING Ids Op Syn)
+       (Import Lord : LORDERED Ids Op Syn)
+       (Import Str : COINDSTREAMS Op OpAux)
+       (Import Sem : LSEMANTICS Ids Op OpAux Syn Lord Str).
+
+  Definition history_tl (H: history) : history := Env.map (@tl value) H.
+
+  Fact history_tl_find : forall (H: history) id vs,
+      Env.find id H = Some vs ->
+      Env.find id (history_tl H) = Some (tl vs).
+  Proof.
+    intros H id vs Hfind.
+    unfold history_tl.
+    rewrite Env.Props.P.F.map_o.
+    rewrite Hfind. reflexivity.
+  Qed.
+
+  Fact history_tl_find_None : forall (H: history) id,
+      Env.find id H = None ->
+      Env.find id (history_tl H) = None.
+  Proof.
+    intros H id Hfind.
+    unfold history_tl.
+    rewrite Env.Props.P.F.map_o.
+    rewrite Hfind. reflexivity.
+  Qed.
+
+  CoInductive sem_clock: history -> Stream bool -> clock -> Stream bool -> Prop :=
+  | Sbase:
+      forall H b b',
+        b ≡ b' ->
+        sem_clock H b Cbase b'
+  | Son:
+      forall H b bk bs ck x k xs c,
+        sem_clock H b ck (true ⋅ bk) ->
+        sem_var H x (present c ⋅ xs) ->
+        val_to_bool c = Some k ->
+        sem_clock (history_tl H) (tl b) (Con ck x k) bs ->
+        sem_clock H b (Con ck x k) (true ⋅ bs)
+  | Son_abs1:
+      forall H b bk bs ck x k xs,
+        sem_clock H b ck (false ⋅ bk) ->
+        sem_var H x (absent ⋅ xs) ->
+        sem_clock (history_tl H) (tl b) (Con ck x k) bs ->
+        sem_clock H b (Con ck x k) (false ⋅ bs)
+  | Son_abs2:
+      forall H b bk bs ck x k c xs,
+        sem_clock H b ck (true ⋅ bk) ->
+        sem_var H x (present c ⋅ xs) ->
+        val_to_bool c = Some k ->
+        sem_clock (history_tl H) (tl b) (Con ck x (negb k)) bs ->
+        sem_clock H b (Con ck x (negb k)) (false ⋅ bs).
+
+  CoInductive synchronized: Stream value -> Stream bool -> Prop :=
+  | synchro_present:
+      forall v vs bs,
+        synchronized vs bs ->
+        synchronized (present v ⋅ vs) (true ⋅ bs)
+  | synchro_absent:
+      forall vs bs,
+        synchronized vs bs ->
+        synchronized (absent ⋅ vs) (false ⋅ bs).
+
+  Fixpoint interp_clock H b cl : Stream bool :=
+    match cl with
+    | Cbase => b
+    | Con cl id b' =>
+      let b := interp_clock H b cl in
+      match Env.find id H with
+      | Some v =>
+        map2 (fun b v => match v with
+                      | OpAux.present v =>
+                        match OpAux.val_to_bool v with
+                        | Some true => andb b b'
+                        | Some false => andb b (negb b')
+                        | _ => false
+                        end
+                      | _ => false
+                      end) b v
+      | None => b
+      end
+    end.
+
+
+  Fact interp_clock_hd : forall cl H b bs,
+      hd (interp_clock H (b ⋅ bs) cl) =
+         match cl with
+         | Cbase => b
+         | Con cl id b' =>
+           let b := hd (interp_clock H (b ⋅ bs) cl) in
+           match Env.find id H with
+           | Some v => match (hd v) with
+                      | present v => match (OpAux.val_to_bool v) with
+                                    | Some true => andb b b'
+                                    | Some false => andb b (negb b')
+                                    | _ => false
+                                    end
+                      | absent => false
+                      end
+           | None => b
+           end
+         end.
+  Proof.
+    induction cl; intros H b0 bs.
+    - reflexivity.
+    - destruct (Env.find i H) eqn:Hfind; simpl.
+      + rewrite Hfind.
+        rewrite <- map2_hd. reflexivity.
+      + simpl. rewrite Hfind. reflexivity.
+  Qed.
+
+  Fact interp_clock_tl : forall cl H bs,
+      tl (interp_clock H bs cl) ≡ interp_clock (history_tl H) (tl bs) cl.
+  Proof.
+    induction cl; intros H bs; simpl in *.
+    - reflexivity.
+    - destruct (Env.find i H) eqn:Hfind.
+      + apply history_tl_find in Hfind. rewrite Hfind.
+        rewrite <- map2_tl. rewrite IHcl. reflexivity.
+      + apply history_tl_find_None in Hfind. rewrite Hfind. auto.
+  Qed.
+
+  Lemma interp_clock_Cons : forall cl H b bs,
+      interp_clock H (b ⋅ bs) cl ≡ hd (interp_clock H (b ⋅ bs) cl) ⋅ (interp_clock (history_tl H) bs cl).
+  Proof.
+    intros cl H b bs.
+    constructor; simpl; auto.
+    symmetry. replace bs with (tl (b ⋅ bs)) at 1; auto.
+    rewrite interp_clock_tl. reflexivity.
+  Qed.
+
+  Fact interp_clock_sound_instant : forall cl H bs bs',
+      sem_clock H bs cl bs' ->
+      hd (interp_clock H bs cl) = hd bs'.
+  Proof with eauto.
+    induction cl; intros H [b0 bs] bs' Hsem; inv Hsem.
+    - inv H1...
+    - eapply IHcl in H4.
+      rewrite interp_clock_hd; simpl.
+      inv H7. eapply Env.find_1 in H1. rewrite H1.
+      rewrite <- H2; simpl. rewrite H9; simpl. rewrite H4; simpl.
+      destruct b...
+    - rewrite interp_clock_hd; simpl.
+      inv H8. eapply Env.find_1 in H1. rewrite H1.
+      rewrite <- H2. reflexivity.
+    - eapply IHcl in H4.
+      rewrite interp_clock_hd; simpl.
+      inv H7. eapply Env.find_1 in H1. rewrite H1.
+      rewrite <- H2; simpl. rewrite H9; simpl. rewrite H4; simpl.
+      destruct k...
+  Qed.
+
+  Lemma interp_clock_sound : forall cl H bs bs',
+      sem_clock H bs cl bs' ->
+      interp_clock H bs cl ≡ bs'.
+  Proof with eauto.
+    cofix interp_clock_sound.
+    intros cl H [b bs] [b' bs'] Hsem.
+    constructor; simpl.
+    - apply interp_clock_sound_instant in Hsem...
+    - inv Hsem.
+      + inv H1...
+      + rewrite interp_clock_tl...
+      + rewrite interp_clock_tl...
+      + rewrite interp_clock_tl...
+  Admitted.
+
+  (* Lemma sem_exp_synchronized : forall G H b e vs, *)
+  (*     sem_exp G H b e vs -> *)
+  (*     Forall2 synchronized vs (List.map (interp_clock H b) (clockof e)). *)
+  (* Proof. *)
+  (*   induction e; intros vs Hsem; inv Hsem. *)
+  (*   - (* const *) *)
+  (*     repeat constructor. *)
+  (*     rewrite H4. *)
+  (* Qed. *)
+End LCLOCKSEMANTICS.
+
+
+Module LClockSemanticsFun
+       (Ids : IDS)
+       (Op : OPERATORS)
+       (OpAux : OPERATORS_AUX Op)
+       (Syn : LSYNTAX Ids Op)
+       (Clo : LCLOCKING Ids Op Syn)
+       (Lord : LORDERED Ids Op Syn)
+       (Str : COINDSTREAMS Op OpAux)
+       (Sem : LSEMANTICS Ids Op OpAux Syn Lord Str) <: LCLOCKSEMANTICS Ids Op OpAux Syn Clo Lord Str Sem.
+  Include LCLOCKSEMANTICS Ids Op OpAux Syn Clo Lord Str Sem.
+End LClockSemanticsFun.
