src/Lustre/Lustre.v
@@ -6,10 +6,12 @@ From Velus Require Export Lustre.LClocking.
 From Velus Require Export Lustre.LTyping.
 From Velus Require Export Lustre.LSemantics.
 From Velus Require Export Lustre.LOrdered.
+From Velus Require Export Lustre.LClockSemantics.
 From Velus Require Export Lustre.Normalization.LNormalization.
 
 From Velus Require Import Common.
 
+Local Set Warnings "-masking-absolute-name".
 Module Type LUSTRE
        (Ids   : IDS)
        (Op    : OPERATORS)
@@ -20,6 +22,7 @@ Module Type LUSTRE
   Declare Module Export Clo: LCLOCKING  Ids Op       Syn.
   Declare Module Export Lord: LORDERED  Ids Op       Syn.
   Declare Module Export Sem: LSEMANTICS Ids Op OpAux Syn Lord Str.
+  Declare Module Export ClockSem : LCLOCKSEMANTICS Ids Op OpAux Syn Clo Lord Str Sem.
   Declare Module Export Norm: LNORMALIZATION Ids Op OpAux Str Syn Typ Clo Lord Sem.
 End LUSTRE.
 
@@ -34,5 +37,6 @@ Module LustreFun
   Module Export Clo := LClockingFun   Ids Op       Syn.
   Module Export Lord:= LOrderedFun    Ids Op       Syn.
   Module Export Sem := LSemanticsFun  Ids Op OpAux Syn Lord Str.
+  Module Export ClockSem := LClockSemanticsFun Ids Op OpAux Syn Clo Lord Str Sem.
   Module Export Norm := LNormalizationFun Ids Op OpAux Str Syn Typ Clo Lord Sem.
 End LustreFun.
